minor change in json interface

compositionality/Json/Json_old.fst
@@ -1,10 +1,10 @@
 module Json
 
-module S = Set_extended
+module S = FStar.Set //Set_extended
 
 let concrete_st_a = int
 
-let concrete_st_b = S.t (pos & nat)
+let concrete_st_b = S.set nat
 
 let init_st_a = 0
 
@@ -12,7 +12,7 @@ let init_st_b = S.empty
 
 let eq_a a b = a = b
 
-let eq_b a b = a == b
+let eq_b a b = S.equal a b
 
 let lem_eq_a a b = ()
 
@@ -23,58 +23,26 @@ type app_op_a : eqtype =
 
 type app_op_b : eqtype =
   |Add : nat -> app_op_b
-  |Rem : nat -> app_op_b
 
 let do_a s o = s + 1
 
-let do_b s o = 
-  match o with
-  |(ts, (rid, Add e)) -> S.add (ts, e) s 
-  |(_, (rid, Rem e)) -> S.filter s (fun ele -> snd ele <> e)
+let do_b s o = let _,(_,Add e) = o in S.add e s
 
-let get_ele (o:op_b) =
-  match snd (snd o) with
-  |Add e -> e
-  |Rem e -> e
-  
+let get_ele (o:op_t{is_beta_op o}) =
+  let (Set _ (Beta_op (Add e))) = snd (snd o) in e
+
 let rc_a o1 o2 = Either
 
-let rc_b o1 o2 = 
-  match snd (snd o1), snd (snd o2) with
-  |Add e1, Rem e2 -> if e1 = e2 then Snd_then_fst else Either
-  |Rem e1, Add e2 -> if e1 = e2 then Fst_then_snd else Either
-  |_ -> Either
+let rc_b o1 o2 = Either
 
 let merge_a l a b = a + b - l
 
-let merge_b l a b = 
-  let da = S.difference a l in    //a - l
-  let db = S.difference b l in    //b - l
-  let i_ab = S.intersection a b in
-  let i_lab = S.intersection l i_ab in   // intersect l a b
-  S.union i_lab (S.union da db)          // (intersect l a b) U (a - l) U (b - l)
+let merge_b l a b = S.union l (S.union a b)
 
 /////////////////////////////////////////////////////////////////////////////
 
-#set-options "--z3rlimit 100 --ifuel 3"
-let rc_non_comm_help1 (o1 o2:op_t)
-  : Lemma (requires distinct_ops o1 o2)
-          (ensures is_beta_op o1 /\ is_beta_op o2 ==>
-                              ((Add? (snd (snd (get_op_b o1))) /\ Rem? (snd (snd (get_op_b o2))) /\ get_ele (get_op_b o1) = get_ele (get_op_b o2) /\ get_key o1 = get_key o2) ==> 
-                              ~ (eq (do (do (init_st (Beta_t (get_key o1))) o1) o2) (do (do (init_st (Beta_t (get_key o1))) o2) o1)))) = ()
-
-let rc_non_comm_help2 (o1 o2:op_t)
-  : Lemma (requires distinct_ops o1 o2)
-          (ensures is_beta_op o1 /\ is_beta_op o2 ==>
-                              ((Rem? (snd (snd (get_op_b o1))) /\ Add? (snd (snd (get_op_b o2))) /\ get_ele (get_op_b o1) = get_ele (get_op_b o2) /\ get_key o1 = get_key o2) ==> 
-                              ~ (eq (do (do (init_st (Beta_t (get_key o1))) o1) o2) (do (do (init_st (Beta_t (get_key o1))) o2) o1)))) = ()
-
-let rc_non_comm (o1 o2:op_t)
-  : Lemma (requires distinct_ops o1 o2)
-          (ensures Either? (rc o1 o2) <==> commutes_with o1 o2) = 
-  rc_non_comm_help1 o1 o2;
-   rc_non_comm_help2 o1 o2
-  
+#set-options "--ifuel 3"
+let rc_non_comm o1 o2 = ()
 let no_rc_chain o1 o2 o3 = ()
 let cond_comm_base s o1 o2 o3 = ()
 let cond_comm_ind s o1 o2 o3 o l = ()
@@ -92,7 +60,7 @@ let base_2op_a o1 o2 = ()
 let base_2op_b o1 o2 = ()
 let base_2op' o1 o2 t = ()
 
-#set-options "--z3rlimit 200 --ifuel 3"
+#set-options "--z3rlimit 100 --ifuel 3"
 let ind_lca_2op_a l o1 o2 ol = ()
 let ind_lca_2op_b l o1 o2 ol = ()
 let ind_lca_2op' l o1 o2 ol = ()
